src/aeq/properties.lean
@@ -34,8 +34,8 @@ theorem self_lift_F_aeq_subst_lift_F (F : X →ν Y) (e : exp X)
     begin /- lam -/
       have H : e ≡α⟨vrel.lift (vname.update a (fresh Y).1 F)⟩ exp.subst.apply (exp.subst.lift (vname.update a (fresh Y).1 F)) e :=
         r (vname.update a (fresh Y).1 F),
-      have P : exp.subst.update_var a (fresh Y).1 (exp.subst.lift F) = exp.subst.lift (vname.update a (fresh Y).1 F) :=
-        funext (exp.subst.update_var_eq_var_update a (fresh Y).1 F),
+      have P : exp.subst.update a (fresh Y).1 (exp.subst.lift F) = exp.subst.lift (vname.update a (fresh Y).1 F) :=
+        funext (exp.subst.update_eq_var_update a (fresh Y).1 F),
       rw [←P] at H,
       exact (lam (map.simple vrel.update.lift H))
     end
@@ -49,40 +49,40 @@ theorem self_aeq_subst_var (e : exp X)
 constant subst_comp.fresh_not_mem.within_lam
 (F : exp.subst X Y) (e : exp (insert a X))
 (r : ∀ {Y : vs V} (F : exp.subst (insert a X) Y),
-  exp.subst.apply (exp.subst.update_var ((fresh (insert a X)).1) (fresh Y).1 F) (exp.insert_var ((fresh (insert a X)).1) e)
+  exp.subst.apply (exp.subst.update ((fresh (insert a X)).1) (fresh Y).1 F) (exp.insert_var ((fresh (insert a X)).1) e)
     ≡α⟨vrel.id (insert (fresh Y).1 Y)⟩
   exp.insert_var (fresh Y).1 (exp.subst.apply F e))
 : exp.subst.apply
-      (exp.subst.update_var a (fresh (insert (fresh Y).1 Y)).1 (exp.subst.update_var (fresh X).1 (fresh Y).1 F))
+      (exp.subst.update a (fresh (insert (fresh Y).1 Y)).1 (exp.subst.update (fresh X).1 (fresh Y).1 F))
       (exp.map (vset.prop_subset_of_insert_comm (fresh X).1 a X) (exp.insert_var (fresh X).1 e))
     ≡α⟨vrel.id (insert (fresh Y).1 Y) ⩁ ((fresh (insert (fresh Y).1 Y)).1, (fresh Y).1)⟩
   exp.map
       (vset.prop_subset_of_insert_comm (fresh Y).1 (fresh Y).1 Y)
-      (exp.insert_var (fresh Y).1 (exp.subst.apply (exp.subst.update_var a (fresh Y).1 F) e))
+      (exp.insert_var (fresh Y).1 (exp.subst.apply (exp.subst.update a (fresh Y).1 F) e))
 
 theorem subst_comp.fresh_not_mem.lam (F : exp.subst X Y) (e : exp (insert a X))
 (r : ∀ {Y : vs V} (F : exp.subst (insert a X) Y),
-  exp.subst.apply (exp.subst.update_var ((fresh (insert a X)).1) (fresh Y).1 F) (exp.insert_var ((fresh (insert a X)).1) e)
+  exp.subst.apply (exp.subst.update ((fresh (insert a X)).1) (fresh Y).1 F) (exp.insert_var ((fresh (insert a X)).1) e)
     ≡α⟨vrel.id (insert (fresh Y).1 Y)⟩
   exp.insert_var (fresh Y).1 (exp.subst.apply F e))
-: exp.subst.apply (exp.subst.update_var (fresh X).1 (fresh Y).1 F) (exp.insert_var (fresh X).1 (exp.lam e))
+: exp.subst.apply (exp.subst.update (fresh X).1 (fresh Y).1 F) (exp.insert_var (fresh X).1 (exp.lam e))
     ≡α⟨vrel.id (insert (fresh Y).1 Y)⟩
   exp.insert_var (fresh Y).1 (exp.subst.apply F (exp.lam e)) :=
   begin
     rw [exp.insert_var.of_lam₂ e],
-    have h : exp.subst.apply (exp.subst.update_var (fresh X).1 (fresh Y).1 F) (exp.lam (exp.map (vset.prop_subset_of_insert_comm (fresh X).1 a X) (exp.insert_var (fresh X).1 e)))
-           = exp.lam (exp.subst.apply (exp.subst.update_var a (fresh (insert (fresh Y).1 Y)).1 (exp.subst.update_var (fresh X).1 (fresh Y).1 F)) (exp.map (vset.prop_subset_of_insert_comm (fresh X).1 a X) (exp.insert_var (fresh X).1 e))) :=
+    have h : exp.subst.apply (exp.subst.update (fresh X).1 (fresh Y).1 F) (exp.lam (exp.map (vset.prop_subset_of_insert_comm (fresh X).1 a X) (exp.insert_var (fresh X).1 e)))
+           = exp.lam (exp.subst.apply (exp.subst.update a (fresh (insert (fresh Y).1 Y)).1 (exp.subst.update (fresh X).1 (fresh Y).1 F)) (exp.map (vset.prop_subset_of_insert_comm (fresh X).1 a X) (exp.insert_var (fresh X).1 e))) :=
       exp.subst.apply.of_lam (exp.map (vset.prop_subset_of_insert_comm (fresh X).1 a X) (exp.insert_var (fresh X).1 e)),
     rw [h], clear h,
     rw [exp.subst.apply.of_lam e],
-    rw [exp.insert_var.of_lam₂ (exp.subst.apply (exp.subst.update_var a (fresh Y).1 F) e)],
+    rw [exp.insert_var.of_lam₂ (exp.subst.apply (exp.subst.update a (fresh Y).1 F) e)],
     apply aeq.lam,
     exact subst_comp.fresh_not_mem.within_lam F e @r
   end
 
 -- Paper: Proposition 6.3 (a)
 theorem subst_comp.fresh_not_mem (F : exp.subst X Y) (e : exp X)
-: exp.subst.apply (exp.subst.update_var (fresh X).1 (fresh Y).1 F) (exp.insert_var (fresh X).1 e)
+: exp.subst.apply (exp.subst.update (fresh X).1 (fresh Y).1 F) (exp.insert_var (fresh X).1 e)
     ≡α⟨vrel.id (insert (fresh Y).1 Y)⟩
   exp.insert_var (fresh Y).1 (exp.subst.apply F e) :=
   begin
@@ -93,7 +93,7 @@ theorem subst_comp.fresh_not_mem (F : exp.subst X Y) (e : exp X)
       generalizing Y F,
     begin /- var -/
       rw [exp.insert_var],
-      simp [exp.map, exp.subst.apply, exp.subst.update_var, exp.subst.update],
+      simp [exp.map, exp.subst.apply, exp.subst.update],
       rw [dif_neg (vname.ne_if_mem_and_not_mem (vname.map_of_subset (vset.prop_subset_refl X) x) (fresh X))],
       cases x with x px,
       exact aeq.refl (exp.insert_var (fresh Y).1 (F ⟨x, px⟩)),
@@ -109,8 +109,8 @@ theorem subst_comp.fresh_not_mem (F : exp.subst X Y) (e : exp X)
 -- Paper: Proposition 6.3 (b)
 theorem subst_comp.extend (a : V) (F : exp.subst X Y) (G : exp.subst Y Z)
 : aeq.extend
-    (exp.subst.apply (exp.subst.update_var (fresh Y).1 (fresh Z).1 G) ∘ exp.subst.update_var a (fresh Y).1 F)
-    (exp.subst.update_var a (fresh Z).1 (exp.subst.apply G ∘ F))
+    (exp.subst.apply (exp.subst.update (fresh Y).1 (fresh Z).1 G) ∘ exp.subst.update a (fresh Y).1 F)
+    (exp.subst.update a (fresh Z).1 (exp.subst.apply G ∘ F))
     (vrel.id (insert a X))
     (vrel.id (insert (fresh Z).1 Z)) :=
   begin
@@ -121,12 +121,12 @@ theorem subst_comp.extend (a : V) (F : exp.subst X Y) (G : exp.subst Y Z)
     cases decidable.em (x = a) with x_eq_a x_ne_a,
     begin /- x_eq_a : x = a -/
       induction x_eq_a,
-      simp [exp.subst.update_var, exp.subst.update, exp.subst.apply],
+      simp [exp.subst.update, exp.subst.apply],
       exact aeq.refl (exp.var (vname.insert_self (fresh Z).1 Z))
     end,
     begin /- x_ne_a : x ≠ a -/
-      rw [exp.subst.update_var_of_ne a (fresh Y).1 F ⟨x, px⟩ x_ne_a],
-      rw [exp.subst.update_var_of_ne a (fresh Z).1 (exp.subst.apply G ∘ F) ⟨x, px⟩ x_ne_a],
+      rw [exp.subst.update_of_ne a (fresh Y).1 F ⟨x, px⟩ x_ne_a],
+      rw [exp.subst.update_of_ne a (fresh Z).1 (exp.subst.apply G ∘ F) ⟨x, px⟩ x_ne_a],
       simp [function.comp],
       exact subst_comp.fresh_not_mem G (F (vname.erase ⟨x, px⟩ x_ne_a))
     end
@@ -134,12 +134,12 @@ theorem subst_comp.extend (a : V) (F : exp.subst X Y) (G : exp.subst Y Z)
 
 -- Paper: Proposition 6.3 (c)
 theorem subst_comp.preservation (F : exp.subst X Y) (G : exp.subst Y Z) (e : exp (insert a X))
-: exp.subst.apply (exp.subst.apply (exp.subst.update_var (fresh Y).1 (fresh Z).1 G) ∘ exp.subst.update_var a (fresh Y).1 F) e
+: exp.subst.apply (exp.subst.apply (exp.subst.update (fresh Y).1 (fresh Z).1 G) ∘ exp.subst.update a (fresh Y).1 F) e
     ≡α⟨vrel.id Z ⩁ ((fresh Z).1, (fresh Z).1)⟩
-  exp.subst.apply (exp.subst.update_var a (fresh Z).1 (exp.subst.apply G ∘ F)) e :=
+  exp.subst.apply (exp.subst.update a (fresh Z).1 (exp.subst.apply G ∘ F)) e :=
   aeq.map.simple (λ z₁ z₂, vrel.is_identity.from_id (vrel.id Z ⩁ ((fresh Z).1, (fresh Z).1))) $
-    aeq.subst_preservation.id (exp.subst.apply (exp.subst.update_var (fresh Y).1 (fresh Z).1 G) ∘ exp.subst.update_var a (fresh Y).1 F)
-                              (exp.subst.update_var a (fresh Z).1 (exp.subst.apply G ∘ F))
+    aeq.subst_preservation.id (exp.subst.apply (exp.subst.update (fresh Y).1 (fresh Z).1 G) ∘ exp.subst.update a (fresh Y).1 F)
+                              (exp.subst.update a (fresh Z).1 (exp.subst.apply G ∘ F))
                               (subst_comp.extend a F G)
                               (aeq.refl e)
 
@@ -149,11 +149,11 @@ theorem subst_comp.lam (F : exp.subst X Y) (G : exp.subst Y Z) (e : exp (insert 
    , exp.subst.apply G (exp.subst.apply F e)
        ≡α⟨vrel.id Z⟩
      exp.subst.apply (exp.subst.apply G ∘ F) e)
-: exp.subst.apply (exp.subst.update_var (fresh Y).1 (fresh Z).1 G) (exp.subst.apply (exp.subst.update_var a (fresh Y).1 F) e)
+: exp.subst.apply (exp.subst.update (fresh Y).1 (fresh Z).1 G) (exp.subst.apply (exp.subst.update a (fresh Y).1 F) e)
     ≡α⟨vrel.id Z ⩁ ((fresh Z).1, (fresh Z).1)⟩
-  exp.subst.apply (exp.subst.update_var a (fresh Z).1 (exp.subst.apply G ∘ F)) e :=
+  exp.subst.apply (exp.subst.update a (fresh Z).1 (exp.subst.apply G ∘ F)) e :=
   aeq.map.simple (λ z₁ z₂, vrel.update.of_id ∘ vrel.is_identity.to_id (insert (fresh Z).1 Z)) $
-    aeq.trans (r (exp.subst.update_var a (fresh Y).1 F) (exp.subst.update_var (fresh Y).1 (fresh Z).1 G))
+    aeq.trans (r (exp.subst.update a (fresh Y).1 F) (exp.subst.update (fresh Y).1 (fresh Z).1 G))
               (subst_comp.preservation F G e)
 
 -- Paper: Proposition 6.3 (e)
