src/exp/subst/properties.lean
@@ -25,18 +25,18 @@ theorem distrib_app (F : subst X Y) (f e : exp X)
 
 -- Substitution distributes over lambda abstraction
 theorem distrib_lam (F : subst X Y) (a : V) (e : exp (insert a X))
-: subst.apply F (lam e) = lam (subst.apply (subst.update_var a (fresh Y).1 F) e) :=
+: subst.apply F (lam e) = lam (subst.apply (subst.update a (fresh Y).1 F) e) :=
   rfl
 
-theorem update_var_of_ne (a b : V) (F : subst X Y) (x : ν∈ insert a X) (p : x.1 ≠ a)
-: subst.update_var a b F x = insert_var b (F (vname.erase x p)) :=
-  by simp [exp.subst.update_var, exp.subst.update, dif_neg p]
+theorem update_of_ne (a b : V) (F : subst X Y) (x : ν∈ insert a X) (p : x.1 ≠ a)
+: subst.update a b F x = insert_var b (F (vname.erase x p)) :=
+  by simp [exp.subst.update, dif_neg p]
 
-theorem update_var_eq_var_update (a b : V) (F : X →ν Y) (x : ν∈ insert a X)
-: subst.update_var a b (subst.lift F) x = subst.lift (vname.update a b F) x :=
+theorem update_eq_var_update (a b : V) (F : X →ν Y) (x : ν∈ insert a X)
+: subst.update a b (subst.lift F) x = subst.lift (vname.update a b F) x :=
   begin
     cases x with c pc,
-    simp [subst.update_var, subst.update, subst.lift, function.comp, vname.update],
+    simp [subst.update, subst.lift, function.comp, vname.update],
     cases decidable.em (c = a) with c_eq_a c_ne_a,
     begin /- c_eq_a : c = a -/
       simp [dif_pos c_eq_a]
@@ -50,12 +50,12 @@ theorem update_var_eq_var_update (a b : V) (F : X →ν Y) (x : ν∈ insert a X
 variables {F G : subst X Y} -- Substitutions
 
 -- Substitution variable update distributes over equality.
-theorem update_var_distrib (a b : V)
+theorem update_distrib (a b : V)
 (P : ∀ (x : ν∈ X), F x = G x) (x : ν∈ insert a X)
-: subst.update_var a b F x = subst.update_var a b G x :=
+: subst.update a b F x = subst.update a b G x :=
   begin
     cases x with c pc,
-    unfold subst.update_var subst.update,
+    simp [subst.update],
     cases decidable.em (c = a) with c_eq_a c_ne_a,
     begin /- c_eq_a : c = a -/
       simp [dif_pos c_eq_a]
@@ -84,7 +84,7 @@ theorem apply_distrib (P : ∀ (x : ν∈ X), F x = G x) (e : exp X)
     end,
     begin /- lam -/
       simp [distrib_lam],
-      rw [r $ update_var_distrib a (fresh Y).1 P],
+      rw [r $ update_distrib a (fresh Y).1 P],
     end
   end
 
